# {index}`Factoring`
by constant and/or variable(s)

## Let's start with some examples

a) $6x^2-x=x(6x-1)$

b) $-8x^4+6=2(-4x^4+3)=-2(4x^4-3)$ Here both are considered valid answers.

c) $20x^3+16x^2+4=4(5x^3+4x^2)+4=4(5x^3+4x^2+1)$ Only products are valid answers.

d) $5xy^2-xy+9y=y\lt(5xy-x+9)$

e) $\frac{9}{2}x^2+\frac{1}{2}x=x(\frac{9}{2}x+\frac{1}{2})=\frac{1}{2}x(9x+1)$

f) $-10a^2b^2+6a^2b-ab=ab(-10ab+6a-1)$

## Factoring by division (can be for quadratic polynomials and higher degrees)

### Examples
a) $P(x)=5x^2-10x-15$

Let's try to find a value for the variable x so that $P(x)=0$.

It turns out that if $x=-1$, then $P(x)=0$. This means that one factor of the polynomial $P(x)$ is $(x+1)$.

Then there are different techniques or algorithms to find out what the other factor will be. I (the author) use a method called a "division angle" since it is an algorithm and it doesn't need "trial and error". Here is a link for the technique used in Finnish schools: <a href="https://opetus.tv/lukio-ops2016/matematiikka/maa2/polynomin-jakaminen-polynomilla-jakokulmassa/" target="_blank">Polynomin jakaminen polynomilla jakokulmassa | Opetus.tv</a>

<iframe width="560" height="315" src="https://www.youtube.com/embed/jNJeZlHsMHg?si=5vpWLdbyo49W-9_C" title="YouTube video player" frameborder="0" allow="accelerometer; autoplay; clipboard-write; encrypted-media; gyroscope; picture-in-picture; web-share" allowfullscreen></iframe>

We found that the second factor is $(5x-15)$, so the polynomial can be factorized as

$P(x)=(x+1)(5x-15)$

But this can be factorized even further! The final answer is $P(x)=5(x+1)(x-3)$ so always remember to factorize as far as possible. With polynomials of higher degree, you have to continue to find out other factors as well.

b) $P(x)=-x^2+4x-3$

One solution for $P(x)=0$ would be $x=1$, since $P(1)=-1^2+4\cdot 1-3=0$. Therefore one factor of $P(x)$ is $x-1$. Let's find the oher factor.

<iframe width="560" height="315" src="https://www.youtube.com/embed/B_NBi4cezd8?si=fvpxlGM7V7ncWGqh" title="YouTube video player" frameborder="0" allow="accelerometer; autoplay; clipboard-write; encrypted-media; gyroscope; picture-in-picture; web-share" allowfullscreen></iframe>

So $P(x)=-x^2+4x-3=(x-1)(-x+3)$.